update

src/encode.v
@@ -1,5 +1,6 @@
 Require Import Bool List Arith Nat.
 Import ListNotations.
+Require Import Mmx.ast_instructions Mmx.binary Mmx.association_list.
 
 Require Import Mmx.ast_instructions.
 Require Import Mmx.binary.
@@ -14,12 +15,32 @@ Definition operand_to_bin (o : operand) : option (list bool) :=
     | reg k => n_bit 8 k
     | empty => n_bit 8 0
   end.
+Definition bin_to_operand (l : list bool) : operand :=
+  match bit_n l with
+  | 0 => empty
+  | n => reg n
+  end.
+    
 
 
-(*
-(* TODO :: here i know that i can always get a binary_instruction but some function don't allow me to 
-return a binary_instruction without encapsulate it into an option type *)
-Definition encode_bis (i : instruction) : option binary_instruction :=
+(* HERE i don't make any garantee about the result if the binary_instruction is to small but i will have some lemma to give it *)
+Fixpoint cut_binary_instruction (bi : binary_instruction) (start : nat) (size : nat) : (list bool) :=
+  match bi with
+  | [] => []
+  | h :: tl => if beq_nat start 0
+               then (if beq_nat size 0 then [] else h :: (cut_binary_instruction tl start (size - 1)))
+               else cut_binary_instruction tl (start -1) size
+  end.
+
+Definition testList := [true ; false ; true ; false ; false ; false ; true ; true ].
+Compute testList.
+Compute cut_binary_instruction testList 5 3.
+
+                 
+
+(* TODO :: here i know that i can always get a binary_instruction but some function don't allow me to  *)
+(* return a binary_instruction without encapsulate it into an option type *)
+Definition encode (i : instruction) : option binary_instruction :=
   match i with
     | mk_instr t op1 op2 op3 =>
       match lookup t encdec with
@@ -40,4 +61,77 @@ Definition encode_bis (i : instruction) : option binary_instruction :=
       end
   end.
 
-*)
+Definition decode (bi : binary_instruction) : option instruction :=
+  match lookdown (bit_n (cut_binary_instruction bi 0 8)) encdec with
+  | Some t =>
+    match t with
+    | tag_n tn => Some (mk_instr t (bin_to_operand (cut_binary_instruction bi 7 8))
+                                 (bin_to_operand (cut_binary_instruction bi 15 8))
+                                 (bin_to_operand (cut_binary_instruction bi 23 8)))
+    | tag_i ti => Some (mk_instr t (bin_to_operand (cut_binary_instruction bi 7 8))
+                                 (bin_to_operand (cut_binary_instruction bi 15 8))
+                                 (immediate (bit_n (cut_binary_instruction bi 23 8))))
+    end
+  | None => None
+  end.
+
+Check instruction.
+
+Lemma encode_size : forall (i : instruction) (bi : binary_instruction), encode i = Some bi -> length bi = 32.
+Proof.
+  intros i bi.
+  induction i.
+  unfold encode.
+  destruct (lookup instr_opcode encdec).
+  -{
+      destruct (n_bit 8 n).
+      -{
+          destruct (operand_to_bin instr_operande1).
+          -{
+              destruct (operand_to_bin instr_operande2).
+              -{
+                  destruct (operand_to_bin instr_operande3).
+                  -{
+                      admit.
+                    }
+                  -discriminate.
+                }
+              -discriminate.
+            }
+            -discriminate.
+        }
+        -discriminate.
+  }
+  -discriminate.
+Admitted.  
+
+
+
+
+Lemma encode_decode : forall (i : instruction) (bi : binary_instruction), encode i = Some bi -> decode bi = Some i.
+Proof.
+  (* why can't i write this ? *)
+(*   assert (I : forall (i : instruction) (bi : binary_instruction), encode i = Some bi ->
+                                                                  lookdown (bit_n (cut_binary_instruction bi 0 8)) = i.instr_opcode). *)
+  induction i.
+  unfold encode.
+  
+Admitted.
+
+
+
+
+
+Example test_instr := mk_instr (tag_i ADD_I) (reg 10) (reg 11) (immediate 12).
+Compute encode test_instr.
+Definition testBoolList := [false; true; false; false; false; false; false; false; false; true; false; true; false; false; false; false; true; true; false; true; false; false; false; false; false; false; true; true; false; false; false; false].
+Compute length testBoolList.
+
+encode test_instr
+
+Compute (match encode test_instr with | Some i => decode i | None => None end).
+  
+
+
+
+
